monae_lib.v
@@ -2,13 +2,14 @@
 (* Copyright (C) 2020 monae authors, license: LGPL-2.1-or-later               *)
 From mathcomp Require Import all_ssreflect.
 From mathcomp Require boolp.
-Require ProofIrrelevance FunctionalExtensionality.
+Require ProofIrrelevance.
 
 Definition proof_irr := boolp.Prop_irrelevance.
 
 Definition eq_rect_eq := @ProofIrrelevance.ProofIrrelevanceTheory.Eq_rect_eq.eq_rect_eq.
 
-Definition fun_ext_dep := @FunctionalExtensionality.functional_extensionality_dep.
+(* TODO: PR to analysis *)
+Definition fun_ext_dep := boolp.functional_extensionality_dep.
 
 (******************************************************************************)
 (*      Shared notations and easy definitions/lemmas of general interest      *)
